knowledge soundness documented

src/KZG_knowledge_soundness.thy
@@ -13,7 +13,23 @@ and thus serve as a strong basis for a proof for the full PLONK version.\<close>
 locale knowledge_sound_game_def = bind_game_proof
 begin
 
+section \<open>Definitions for the knowledge soundness game\<close>
+
+text \<open>We define the knowledge soundness game, the reduction to the evaluation binding game and thus 
+transitively to the t-SDH assumption as well as any functions needed to construct them in this locale. 
+This file contains another locale below which contains the proof.\<close>
+
 subsection \<open>Game definition\<close>
+
+text \<open>Note, the adversary for the knowledge soundness is in the Algebraic Group Model (AGM) and 
+thus has to provide a vector we typed `calc_vector` for every group element it outputs. Furthermore, 
+the group elements must be a linear combination of the group elements the adversary has seen so far.
+the vector indicates the parameters of the linear combination. Intuitively, for e.g.
+seen group elements (3,2,1), the adversary could create the value 5 with the vector (0,2,1) as 
+5 = 3*0+2*2+1*1.\<close>
+
+text \<open>Furthermore, the adversary for knowledge soundness is split up into two parts A=(A',A'') 
+that share a state.\<close>
 
 type_synonym '\<sigma>' state = '\<sigma>'
 
@@ -27,10 +43,15 @@ type_synonym ('a', 'e', '\<sigma>')  adversary_2 =
   "'\<sigma>' state \<Rightarrow> 'a' pk \<Rightarrow> 'a' commit \<Rightarrow> 'e' calc_vector \<Rightarrow> 
    ('e' eval_position \<times> 'e' eval_value \<times> 'a' eval_witness) spmf"
 
+text \<open>The extractor is an algorithm that plays against the adversary. It is granted access to the 
+adversaries messages and state (which we neglect in this case as we do not need it because the 
+calculation vector is enough to create sensible values) and has to come up with a polynomial such 
+that the adversary cannot create valid opening points that are not part of the polynomial.\<close>
 type_synonym ('a', 'e') extractor = 
   "'a' commit \<Rightarrow> 'e' calc_vector \<Rightarrow> 
     'e' mod_ring poly"
 
+text \<open>This is the formalized knowledge soundness game\<close>
 definition knowledge_soundness_game :: "('a, 'e) extractor \<Rightarrow> ('a, 'e, '\<sigma>) adversary_1 \<Rightarrow> ('a, 'e, '\<sigma>) adversary_2 
   \<Rightarrow> bool spmf"
   where "knowledge_soundness_game E \<A> \<A>' = TRY do {
@@ -43,16 +64,47 @@ definition knowledge_soundness_game :: "('a, 'e) extractor \<Rightarrow> ('a, 'e
   _ ::unit \<leftarrow> assert_spmf (valid_msg \<phi>_i w_i);
   return_spmf (VerifyEval PK C i \<phi>_i w_i \<and> \<phi>_i \<noteq> poly \<phi> i)} ELSE return_spmf False"
 
+text \<open>The advantage of the adversary over the knowledge soundness game is the probabillity that it 
+wins.\<close>
 definition knowledge_soundness_game_advantage :: "('a, 'e) extractor \<Rightarrow> ('a, 'e, '\<sigma>) adversary_1 \<Rightarrow> ('a, 'e, '\<sigma>) adversary_2 
    \<Rightarrow> real"
   where "knowledge_soundness_game_advantage E \<A> \<A>' \<equiv> spmf (knowledge_soundness_game E \<A> \<A>') True"
 
-subsubsection \<open>reduction definition\<close>
+subsection \<open>reduction definition\<close>
 
+text \<open>The reduction function takes a adversary for the knowledge soundess game and returns an 
+adversary for the evaluation binding game. Specifically, the reduction uses the knowledge soundness 
+adversary to construct a winning strategy for the evaluation binding game (i.e. to win it every 
+time).
+Essentially, it uses the fact that the values supplied by the adversary already break the binding 
+game.\<close>
 definition knowledge_soundness_reduction
   :: "('a, 'e) extractor \<Rightarrow> ('a, 'e, '\<sigma>) adversary_1 \<Rightarrow> ('a, 'e, '\<sigma>) adversary_2 \<Rightarrow> ('a, 'e) adversary"                     
 where
   "knowledge_soundness_reduction E \<A> \<A>' PK = do {
+  (C,calc_vec, \<sigma>) \<leftarrow> \<A> PK; 
+  let \<phi> = E C calc_vec;
+  (i, \<phi>_i, w_i) \<leftarrow> \<A>' \<sigma> PK C calc_vec;
+  let \<phi>'_i = poly \<phi> i;
+  let w'_i = createWitness PK \<phi> i;
+  return_spmf (C, i, \<phi>_i, w_i, \<phi>'_i, w'_i)}"
+
+end
+
+text \<open>This locale captures the proof for the definitions provided earlier\<close>
+locale knowledge_sound_game_proof = knowledge_sound_game_def
+begin
+
+subsection \<open>helping definitions\<close>
+
+text \<open>The knowledge soundness reduction adversary extended for asserts that 
+are present in the evaluation binding game. We use this definition to show equivalence to 
+the evaluation binding game. Later on we can then easily over-estimate the probability from 
+this extended version to the normal reduction.\<close>
+definition knowledge_soundness_reduction_ext
+  :: "('a, 'e) extractor \<Rightarrow> ('a, 'e, '\<sigma>) adversary_1 \<Rightarrow> ('a, 'e, '\<sigma>) adversary_2 \<Rightarrow> ('a, 'e) adversary"                     
+where
+  "knowledge_soundness_reduction_ext E \<A> \<A>' PK = do {
   (C,calc_vec, \<sigma>) \<leftarrow> \<A> PK;
   _ :: unit \<leftarrow> assert_spmf (length PK = length calc_vec 
                           \<and> C = fold (\<lambda> i acc. acc \<otimes>\<^bsub>G\<^sub>p\<^esub> PK!i ^\<^bsub>G\<^sub>p\<^esub> (calc_vec!i)) [0..<length PK] \<one>\<^bsub>G\<^sub>p\<^esub>);  
@@ -63,11 +115,19 @@ where
   let w'_i = createWitness PK \<phi> i;
   return_spmf (C, i, \<phi>_i, w_i, \<phi>'_i, w'_i)}"
 
-subsubsection \<open>Extractor definition\<close>
+text \<open>Extractor definition\<close>
 fun E :: "('a, 'e) extractor" where 
   "E C calc_vec = Poly calc_vec"
 
-subsubsection \<open>alternative definitions for easier proving + their equivalence proofs\<close>
+lemma key_gen_alt_def: "KeyGen = do {
+    x :: nat \<leftarrow> sample_uniform (order G\<^sub>p);
+    let \<alpha>::'e mod_ring = of_int_mod_ring (int x) in
+    return_spmf (map (\<lambda>t. \<^bold>g\<^bsub>G\<^sub>p\<^esub> ^\<^bsub>G\<^sub>p\<^esub> (\<alpha>^t)) [0..<max_deg+1])
+  }"
+  unfolding KeyGen_def Setup_def Let_def split_def by simp
+
+
+subsection \<open>literal helping lemmas\<close>
 
 lemma pull_down_assert_spmf_with_return:
 "do {
@@ -129,13 +189,32 @@ proof -
   then show ?thesis by presburger
 qed
 
-lemma key_gen_alt_def: "KeyGen = do {
-    x :: nat \<leftarrow> sample_uniform (order G\<^sub>p);
-    let \<alpha>::'e mod_ring = of_int_mod_ring (int x) in
-    return_spmf (map (\<lambda>t. \<^bold>g\<^bsub>G\<^sub>p\<^esub> ^\<^bsub>G\<^sub>p\<^esub> (\<alpha>^t)) [0..<max_deg+1])
-  }"
-  unfolding KeyGen_def Setup_def Let_def split_def by simp
+subsection \<open>Reduction proof\<close>
 
+text \<open>We structure the proof in 5 parts:
+
+1. We restate the knowledge soundness game such that all assert statements are combined in one.
+
+2. We restate the evaluation binding game with the extended reduction adversary such that all 
+assert statements are combined in one.
+
+3. We show that the accumulated assert statements in the last two steps are equivalent. Furthermore, 
+we can conclude that the games are in fact equivalent.
+
+4. We conclude from step 1 to 3 that the knowledge soundness game is the same game as the evalutaion 
+binding game for the extended adversary
+
+5. We overestimate the extended reduction with the normal reduction.
+
+6. We conclude from step 4 that the probability of winning the knowledge soundness game is less 
+than or equal to winning the evaluation binding game with the normal reduction adversary. 
+Furthermore, we can conclude transitively through the evaluation binding game, that the probability 
+of the adversary winning the knowledge soundness game is less than or equal to breaking the 
+t-SDH assumption.
+\<close>
+
+
+text \<open>Proof Step 1:\<close>
 lemma knowledge_soundness_game_alt_def: 
   "knowledge_soundness_game E \<A> \<A>' = 
    TRY do {
@@ -153,6 +232,9 @@ lemma knowledge_soundness_game_alt_def:
   } ELSE return_spmf False"
 proof -
   note [simp] = Let_def split_def
+
+  text \<open>we rearrange the asserts together in the knowledge soundness game so that we can combine 
+  them later on.\<close>
   have "do {
   PK \<leftarrow> KeyGen;
   (C,calc_vec, \<sigma>) \<leftarrow> \<A> PK;
@@ -183,6 +265,7 @@ proof -
     return_spmf (VerifyEval PK C i \<phi>_i w_i \<and> \<phi>_i \<noteq> poly \<phi> i)
   } ELSE return_spmf False"
     unfolding knowledge_soundness_game_def by algebra
+  text \<open>Now we unfold the knowledge soundness game to merge multiple asserts together.\<close>
   also have "\<dots> = TRY do {
     PK \<leftarrow> KeyGen;
     TRY do {
@@ -205,6 +288,7 @@ proof -
   } ELSE return_spmf False"
    unfolding split_def Let_def
    by (fold try_bind_spmf_lossless2[OF lossless_return_spmf])simp
+  text \<open>However, before merging we turn the return statement into another assert\<close>
   also have "\<dots> = TRY do {
     PK \<leftarrow> KeyGen;
     TRY do {
@@ -226,7 +310,8 @@ proof -
     } ELSE return_spmf False
     } ELSE return_spmf False
   } ELSE return_spmf False"
-   by(auto simp add: try_bind_assert_spmf try_spmf_return_spmf1 intro!: try_spmf_cong bind_spmf_cong)
+    by(auto simp add: try_bind_assert_spmf try_spmf_return_spmf1 intro!: try_spmf_cong bind_spmf_cong)
+  text \<open>Now we add the first two asserts together\<close>
   also have "\<dots> = TRY do {
     PK \<leftarrow> KeyGen;
     TRY do {
@@ -249,6 +334,7 @@ proof -
     } ELSE return_spmf False
   } ELSE return_spmf False"
     using assert_anding by presburger
+  text \<open>we fold again to merge the remaining asserts\<close>
    also have "\<dots> = TRY do {
     PK \<leftarrow> KeyGen;
     TRY do {
@@ -270,6 +356,7 @@ proof -
   } ELSE return_spmf False"
     unfolding split_def Let_def
     by(fold try_bind_spmf_lossless2[OF lossless_return_spmf]) simp
+  text \<open>Now we can merge the remaining two asserts\<close>
    also have "\<dots> = TRY do {
     PK \<leftarrow> KeyGen;
     TRY do {
@@ -290,7 +377,9 @@ proof -
     } ELSE return_spmf False
   } ELSE return_spmf False"
      using assert_anding by presburger
-   text \<open>next step, add assert PK construction\<close>
+   text \<open>next we want to make the construction of PK accessible in the assert. 
+    For that we have to take two steps. Firstly we have unfold KeyGen to obtain access to the 
+    computation of PK.\<close>
   also have "\<dots> = TRY do {
     x :: nat \<leftarrow> sample_uniform (order G\<^sub>p);
     let \<alpha> = of_int_mod_ring (int x);
@@ -314,6 +403,9 @@ proof -
   } ELSE return_spmf False"
      using key_gen_alt_def
      by (smt (verit, ccfv_SIG) bind_spmf_assoc bind_spmf_cong)
+   text \<open>Secondly, we have to unwrap the definition of PK from the spmf into a constant one. 
+   If PK is constant, we can drag its definition into the assert, instead of the variable 
+   PK.\<close>
     also have "\<dots> = TRY do {
     x :: nat \<leftarrow> sample_uniform (order G\<^sub>p);
     let \<alpha> = of_int_mod_ring (int x);
@@ -336,6 +428,7 @@ proof -
     } ELSE return_spmf False
   } ELSE return_spmf False"
       using return_bind_spmf by meson
+  text \<open>Lastly we fold the game together to obtain a clean game with all asserts accumulated.\<close>
   also have "\<dots> = TRY do {
     x :: nat \<leftarrow> sample_uniform (order G\<^sub>p);
     let \<alpha> = of_int_mod_ring (int x);
@@ -354,8 +447,9 @@ proof -
   finally show ?thesis .
 qed
 
+text \<open>Proof Step 2:\<close>
 lemma bind_game_knowledge_soundness_reduction_alt_def: 
-  "bind_game (knowledge_soundness_reduction E \<A> \<A>') = 
+  "bind_game (knowledge_soundness_reduction_ext E \<A> \<A>') = 
   TRY do {
     x :: nat \<leftarrow> sample_uniform (order G\<^sub>p);
     let \<alpha> = of_int_mod_ring (int x);
@@ -374,15 +468,18 @@ lemma bind_game_knowledge_soundness_reduction_alt_def:
        return_spmf True
     } ELSE return_spmf False"
 proof -
-  have "bind_game (knowledge_soundness_reduction E \<A> \<A>') = TRY do {
+  text \<open>Firstly we extract the return value from the evaluation binding game into a assert statement.\<close>
+  have "bind_game (knowledge_soundness_reduction_ext E \<A> \<A>') = TRY do {
   PK \<leftarrow> KeyGen;
-  (C, i, \<phi>_i, w_i, \<phi>'_i, w'_i) \<leftarrow> (knowledge_soundness_reduction E \<A> \<A>') PK;
+  (C, i, \<phi>_i, w_i, \<phi>'_i, w'_i) \<leftarrow> (knowledge_soundness_reduction_ext E \<A> \<A>') PK;
   _ :: unit \<leftarrow> assert_spmf (\<phi>_i \<noteq> \<phi>'_i \<and> valid_msg \<phi>_i w_i \<and> valid_msg \<phi>'_i w'_i);
   let b = VerifyEval PK C i \<phi>_i w_i;
   let b' = VerifyEval PK C i \<phi>'_i w'_i;
   _ :: unit \<leftarrow> assert_spmf (b \<and> b');
   return_spmf True } ELSE return_spmf False" 
     by (fact bind_game_alt_def)
+  text \<open>Secondly, we inline the extended knowledge soundness adversary, so we can accumulate
+  the asserts from the reduction and the game together.\<close>
   also have "\<dots> = TRY do {
   PK \<leftarrow> KeyGen;
   (C,calc_vec, \<sigma>) \<leftarrow> \<A> PK;
@@ -398,7 +495,8 @@ proof -
   let b' = VerifyEval PK C i \<phi>'_i w'_i;
   _ :: unit \<leftarrow> assert_spmf (b \<and> b');
   return_spmf True } ELSE return_spmf False"
-  unfolding knowledge_soundness_reduction_def by (simp add: split_def Let_def)
+  unfolding knowledge_soundness_reduction_ext_def by (simp add: split_def Let_def)
+  text \<open>We fold the game into smaller sub games, such that we can combine the individual asserts.\<close>
   also have "\<dots> =  TRY do {
     PK \<leftarrow> KeyGen;
     TRY do {
@@ -427,6 +525,7 @@ proof -
     } ELSE return_spmf False"
    unfolding split_def Let_def 
    by(fold try_bind_spmf_lossless2[OF lossless_return_spmf]) simp
+ text \<open>We combine the first two asserts\<close>
   also have "\<dots> = TRY do {
     PK \<leftarrow> KeyGen;
     TRY do {
@@ -455,6 +554,7 @@ proof -
     } ELSE return_spmf False
     } ELSE return_spmf False"
     using assert_anding by presburger
+  text \<open>WE fold again to accumulate the next two asserts\<close>  
   also have "\<dots> = TRY do {
     PK \<leftarrow> KeyGen;
     TRY do {
@@ -482,6 +582,7 @@ proof -
     } ELSE return_spmf False"
    unfolding split_def Let_def 
    by(fold try_bind_spmf_lossless2[OF lossless_return_spmf]) simp
+ text \<open>We merge the next two asserts, but omit repeated checks\<close>
   also have "\<dots> = TRY do {
     PK \<leftarrow> KeyGen;
     TRY do {
@@ -522,6 +623,8 @@ proof -
       by meson
     then show ?thesis using assert_anding by algebra
   qed
+  text \<open>We fold the game into one coherent game again to rearrange asserts.
+  We aim to bring the asserts closer together so we can merge them.\<close>
   also have "\<dots> =  TRY do {
     PK \<leftarrow> KeyGen;
     (C,calc_vec, \<sigma>) \<leftarrow> \<A> PK;
@@ -580,6 +683,8 @@ proof -
       by (simp add: Let_def split_def)
     then show ?thesis by argo
   qed
+  text \<open>We unfold the game again into smaller sub games, so we can accumulate the rearranged assert 
+  as well.\<close>
   also have "\<dots> =  TRY do {
     PK \<leftarrow> KeyGen;
     TRY do {
@@ -601,6 +706,7 @@ proof -
     } ELSE return_spmf False"
   unfolding split_def Let_def 
   by(fold try_bind_spmf_lossless2[OF lossless_return_spmf]) simp
+  text \<open>We accumulate the last assert\<close>
   also have "\<dots> = TRY do {
     PK \<leftarrow> KeyGen;
     TRY do {
@@ -621,6 +727,7 @@ proof -
     } ELSE return_spmf False
     } ELSE return_spmf False"
     using assert_anding by presburger
+  text \<open>We fold the sub games together to one clean coherent game.\<close>
   also have "\<dots> = TRY do {
     PK \<leftarrow> KeyGen;
     (C,calc_vec, \<sigma>) \<leftarrow> \<A> PK;
@@ -637,7 +744,8 @@ proof -
     } ELSE return_spmf False"
    unfolding split_def Let_def 
    by(fold try_bind_spmf_lossless2[OF lossless_return_spmf]) simp
- text \<open>make PK definition extractable\<close>
+ text \<open>Similarly to the prior lemma, we want to make PK accessible in the assert statement and thus
+  we unfold KeyGen to reveal the computation of PK.\<close>
   also have "\<dots> = TRY do {
     x :: nat \<leftarrow> sample_uniform (order G\<^sub>p);
     let \<alpha> = of_int_mod_ring (int x);
@@ -656,6 +764,7 @@ proof -
     } ELSE return_spmf False"
     using key_gen_alt_def
     by (smt (verit, ccfv_SIG) bind_spmf_assoc bind_spmf_cong)
+  text \<open>Secondly, we extract the definition of PK out of the spmf into a constant one.\<close>
   also have "\<dots> = TRY do {
     x :: nat \<leftarrow> sample_uniform (order G\<^sub>p);
     let \<alpha> = of_int_mod_ring (int x);
@@ -673,6 +782,9 @@ proof -
        return_spmf True
     } ELSE return_spmf False"
     using return_bind_spmf by meson
+  text \<open>Lastly we add a statement implied by the other statement in the assert, namely that the 
+  witness w_i cannot be equal to `createWitness PK \<phi> i`. This will allow for easier reasoning about 
+  the equivalence of the asserts in the next step.\<close>
   also have "\<dots> = TRY do {
     x :: nat \<leftarrow> sample_uniform (order G\<^sub>p);
     let \<alpha> = of_int_mod_ring (int x);
@@ -694,8 +806,6 @@ proof -
   finally show ?thesis .
 qed
 
-subsection \<open>Reduction proof\<close>
-
 lemma fold_split:"i\<le>n \<Longrightarrow> fold f [0..<n] init = fold f [i..<n] (fold f [0..<i] init)"
 proof -
   assume asm: "i\<le>n"
@@ -706,7 +816,9 @@ proof -
   finally show "fold f [0..<n] init = fold f [i..<n] (fold f [0..<i] init)" .
 qed
 
-text \<open>show the equivalence of the content of the assert statements in the alt games i.e. 
+text \<open>Proof Step 3:
+
+We show the equivalence of the content of the assert statements in the alt games i.e.
 assert content of knowledge_soundness_game_alt_def
 is equivalent to the 
 assert content of bind_game_knowledge_soundness_reduction_alt_def\<close>
@@ -727,6 +839,7 @@ lemma asserts_are_equal:
 proof 
   let ?PK = "(map (\<lambda>t. \<^bold>g\<^bsub>G\<^sub>p\<^esub> ^\<^bsub>G\<^sub>p\<^esub> (\<alpha>^t)) [0..<max_deg+1])"
   let ?\<phi> = "Poly calc_vec"
+
   assume asm: "length ?PK = length calc_vec 
             \<and> C = fold (\<lambda> i acc. acc \<otimes>\<^bsub>G\<^sub>p\<^esub> ?PK!i ^\<^bsub>G\<^sub>p\<^esub> (calc_vec!i)) [0..<length ?PK] \<one>\<^bsub>G\<^sub>p\<^esub>
             \<and> valid_msg \<phi>_i w_i 
@@ -953,20 +1066,86 @@ proof
   qed (simp add: asm)+
 qed linarith
 
-theorem knowledge_soundness_game_eq_bind_game_knowledge_soundness_reduction: 
-  "knowledge_soundness_game E \<A> \<A>' = bind_game (knowledge_soundness_reduction E \<A> \<A>')"
+text \<open>Proof step 4:\<close>
+
+text \<open>From the last three steps, we conclude that the know,ledge_soundness_game is the same game as 
+the evaluation binding game for the extended reduction adversary.\<close>
+lemma knowledge_soundness_game_eq_bind_game_knowledge_soundness_reduction_ext: 
+  "knowledge_soundness_game E \<A> \<A>' = bind_game (knowledge_soundness_reduction_ext E \<A> \<A>')"
   unfolding knowledge_soundness_game_alt_def 
             bind_game_knowledge_soundness_reduction_alt_def
             Let_def
   using asserts_are_equal by simp
 
-theorem evaluation_knowledge_soundness: 
+text \<open>Proof Step 5:
+
+We overestimate the probability of winning the evaluation binding game with the extended adversary 
+by winning it with the normal adversary.\<close>
+lemma overestimate_reductions: "spmf (bind_game (knowledge_soundness_reduction_ext E \<A> \<A>')) True 
+  \<le> spmf (bind_game (knowledge_soundness_reduction E \<A> \<A>')) True"
+proof -
+   note [simp] = Let_def split_def
+
+   have w_assert_ext: "bind_game (knowledge_soundness_reduction_ext E \<A> \<A>') = TRY do {
+    PK \<leftarrow> KeyGen;
+    (C,calc_vec, \<sigma>) \<leftarrow> \<A> PK;
+    _ :: unit \<leftarrow> assert_spmf (length PK = length calc_vec 
+                            \<and> C = fold (\<lambda> i acc. acc \<otimes>\<^bsub>G\<^sub>p\<^esub> PK!i ^\<^bsub>G\<^sub>p\<^esub> (calc_vec!i)) [0..<length PK] \<one>\<^bsub>G\<^sub>p\<^esub>);  
+    let \<phi> = E C calc_vec;
+    (i, \<phi>_i, w_i) \<leftarrow> \<A>' \<sigma> PK C calc_vec;
+    _ :: unit \<leftarrow> assert_spmf (valid_msg \<phi>_i w_i);
+    let \<phi>'_i = poly \<phi> i;
+    let w'_i = createWitness PK \<phi> i;
+    _ :: unit \<leftarrow> assert_spmf (\<phi>_i \<noteq> \<phi>'_i \<and> valid_msg \<phi>_i w_i \<and> valid_msg \<phi>'_i w'_i);
+    let b = VerifyEval PK C i \<phi>_i w_i;
+    let b' = VerifyEval PK C i \<phi>'_i w'_i;
+    _ :: unit \<leftarrow> assert_spmf (b \<and> b');
+    return_spmf True } ELSE return_spmf False"
+     unfolding bind_game_alt_def knowledge_soundness_reduction_ext_def 
+     by (simp add: split_def Let_def)
+
+   have wo_assert_ext: "bind_game (knowledge_soundness_reduction E \<A> \<A>') = TRY do {
+    PK \<leftarrow> KeyGen;
+    (C,calc_vec, \<sigma>) \<leftarrow> \<A> PK;
+    let \<phi> = E C calc_vec;
+    (i, \<phi>_i, w_i) \<leftarrow> \<A>' \<sigma> PK C calc_vec;
+    let \<phi>'_i = poly \<phi> i;
+    let w'_i = createWitness PK \<phi> i;
+    _ :: unit \<leftarrow> assert_spmf (\<phi>_i \<noteq> \<phi>'_i \<and> valid_msg \<phi>_i w_i \<and> valid_msg \<phi>'_i w'_i);
+    let b = VerifyEval PK C i \<phi>_i w_i;
+    let b' = VerifyEval PK C i \<phi>'_i w'_i;
+    _ :: unit \<leftarrow> assert_spmf (b \<and> b');
+    return_spmf True } ELSE return_spmf False"
+     unfolding bind_game_alt_def knowledge_soundness_reduction_def 
+     by (simp add: split_def Let_def)
+
+  text \<open>We show the thesis in ennreal, which implies the plain thesis\<close>
+  have "ennreal (spmf (bind_game (knowledge_soundness_reduction_ext E \<A> \<A>')) True) 
+    \<le> ennreal (spmf (bind_game (knowledge_soundness_reduction E \<A> \<A>')) True)"
+    unfolding w_assert_ext wo_assert_ext
+    apply (simp add: spmf_try_spmf ennreal_spmf_bind)
+    apply (rule nn_integral_mono)+
+    apply (simp add: assert_spmf_def)
+    apply (simp add: measure_spmf.emeasure_eq_measure)
+    apply (simp add: mult_left_le nn_integral_mono)
+    done
+    
+  then show ?thesis by simp
+qed
+  
+text \<open>Proof Step 6:
+
+Finally we put everything together:
+we conclude that for every efficient adversary in the AGM the advantage of winning the 
+knowledge soundness game is less equal to breaking the t-SDH assumption.\<close>
+theorem knowledge_soundness: 
   "knowledge_soundness_game_advantage E \<A> \<A>' 
-  = t_SDH_G\<^sub>p.advantage (bind_reduction (knowledge_soundness_reduction E \<A> \<A>'))"
-  using knowledge_soundness_game_eq_bind_game_knowledge_soundness_reduction 
-        evaluation_binding
-  unfolding bind_advantage_def knowledge_soundness_game_advantage_def
-  by metis
+  \<le> t_SDH_G\<^sub>p.advantage (eval_bind_reduction (knowledge_soundness_reduction E \<A> \<A>'))"
+  using evaluation_binding[of "knowledge_soundness_reduction E \<A> \<A>'"]
+    overestimate_reductions[of \<A> \<A>']
+  unfolding bind_advantage_def knowledge_soundness_game_advantage_def 
+  unfolding knowledge_soundness_game_eq_bind_game_knowledge_soundness_reduction_ext
+  by linarith
 
 end
 
